Experiments.v
@@ -1,0 +1,209 @@
+(** * Experiments. *)
+
+(** This file has material from LDef.v and LProps.v that I've experiemnted with 
+    and needs more investigation. *)
+
+Load Init.
+Require Export SfLib.
+Require Import LibTactics.
+
+Require Export Common LDef LProps.
+Import P3Common LDEF LProps.
+
+(* TBD: Try some of these attempts at making the lookup stuff more generic:
+
+Definition lookup_generic {T U : Type} 
+    (extrf : T -> option U) (xs : list T) : option U := 
+  match xs with 
+    | nil => None
+    | x :: xs' => 
+      match extrf x with
+        | None => lookup_generic extrf xs'
+        | Some v => Some v
+      end
+  end.
+
+Definition vdef_xf (x : id) (vd : def) : option tm :=
+  match vd with 
+    | (Vd y t) => if id_eq_dec x y then Some t else None
+    | _ => None
+  end.
+Definition lookup_vdef x Fs := lookup_generic (vdef_xf x) Fs.
+
+Definition unapply_vdef (vd : vdef) : option (id * tm) :=
+  match vd with (Fv y t) => Some (y, t) | _ => None end.
+  
+Definition lookup_gen {T U : Type} (unapplyf : T -> option (id * U)) 
+    (x : id) (ts : list T) : option U :=
+  match ts with
+    | nil => None
+    | t : ts' => 
+      match unapplyf t with
+        | Some (y v) => 
+            if id_eq_dec x y then Some v else lookup_gen unapplyf x ts'
+        | None => lookup_gen unapplyf x ts'
+      end
+  end.
+Definition lookup_vdef := lookup_gen unapply_vdef.
+*)
+
+(* Here is a version of [ty_xrect] that uses the underlying recursion principles,
+   [ty_rect] and [list_rect].
+*)
+
+Definition ty_xrect'
+  (P: ty -> Type) 
+  (Q: list decl -> Type)
+    (fTBase : forall x : id, P (TBase x))
+    (fTBool : P (TBool))
+    (fTArrow : forall T1 : ty, P T1 -> forall T2 : ty, P T2 -> P (TArrow T1 T2))
+    (fTRcd' : forall Trb : list decl, Q Trb -> P (TRcd Trb))
+      (fTRcd_nil' : Q nil)
+      (fTRcd_cons' : forall (x : id) (T : ty) (Trb : list decl), 
+                       P T -> Q Trb -> Q ((Lv x T) :: Trb))
+  : forall T : ty, P T
+  := fix F (T : ty) : P T :=
+    let fTRcd_cons b Trb := 
+      match b with (Lv x T) => fTRcd_cons' x T Trb (F T) end
+    in let fTRcd Trb := fTRcd' Trb (list_rect Q fTRcd_nil' fTRcd_cons Trb)
+    in ty_rect P fTBase fTBool fTArrow fTRcd T.
+
+(* This doesn't work:
+  := fix F (T : ty) {struct T} : P T :=
+     match T as T0 return (P T0) with
+       | TBase x => fTBase x
+       | TBool => fTBool
+       | TArrow T1 T2 => fTArrow T1 (F T1) T2 (F T2)
+       | TRcd Trb => fTRcd' Trb (G Trb)
+     end
+   with G (Trb : list decl) {struct Trb} : Q Trb :=
+     match Trb as Trb0 return (Q Trb0) with
+       | nil => fTRcd_nil'
+       | (Lv x T) :: Trb' => fTRcd_cons' x T Trb' (F T) (G Trb')
+     end
+   for F.
+*)
+
+(* An attempt to do it as a Lemma, but the lack of a good IH kills it.
+
+Lemma ty_xrect'' :
+  forall 
+    (P: ty -> Type) 
+    (Q: list decl -> Type),
+    (forall x : id, P (TBase x)) ->
+    (forall T1 : ty, P T1 -> forall T2 : ty, P T2 -> P (TArrow T1 T2)) ->
+    (forall Trb : list decl, Q Trb -> P (TRcd Trb)) ->
+      (Q nil) ->
+      (forall (x : id) (T : ty) (Trb : list decl), 
+           P T -> Q Trb -> Q ((x, T) :: Trb)) ->
+  forall T : ty, P T.
+Proof.
+  intros P Q Hbase Harrow Hrcd Hnil Hcons T.
+  T_cases (induction T) Case; auto.
+    Case "TRcd". (* no IH *) apply Hrcd. induction a; auto.
+      SCase "cons". destruct a as [x T]. apply Hcons. (* Can't prove P T *)
+Abort All.
+*)
+
+(** It would be nice if one did not have to specify Q at the start, 
+    but rather when it comes up in the TRcd case. *)
+(*
+Definition ty_xrect_plus
+  (P: ty -> Type) 
+    (fTBase : forall x : id, P (TBase x))
+    (fTArrow : forall T1 : ty, P T1 -> forall T2 : ty, P T2 -> P (TArrow T1 T2))
+    (fTRcd : forall Trb : list decl, 
+      (exists (Q: list decl -> Type),
+              (Q nil) *
+              (forall (x : id) (T : ty) (Trb : list decl), 
+                       P T -> Q Trb -> Q ((x, T) :: Trb)) *
+              (forall Trb : list decl, (Q Trb) -> P (TRcd Trb)) ???
+      ) -> P (TRcd Trb))   
+  : forall T : ty, P T := admit.
+  := fix F (T : ty) : P T :=
+     let fix G (Trb : list decl) : Q Trb :=
+         match Trb with
+           | nil => fTRcd_nil'
+           | (x,T) :: Trb' => fTRcd_cons' x T Trb' (F T) (G Trb')
+         end
+     in match T with
+       | TBase x => fTBase x
+       | TArrow T1 T2 => fTArrow T1 (F T1) T2 (F T2)
+       | TRcd Trb => fTRcd' Trb (G Trb)
+     end.
+*)
+
+(**   Here is substitution defined using the custom recursion defined in [LDef.v].
+      However, I don't know how to use the match syntax with a custom 
+      recursion principle, so it's not easy to read.  Further, it simplifies 
+      into a mess that I can't fold back up, so I'm not using it. *)
+
+Definition subst_ugly (x:id) (s:tm) :tm -> tm := 
+  tm_xrect (fun _ => tm) (fun _ => list def)
+    ttrue                                               (* ttrue *)
+    tfalse                                              (* tfalse *)
+    (fun y => if eq_id_dec x y then s else (tvar y))    (* tvar y *)
+    (fun t1 mt1 t2 mt2 => tapp mt1 mt2)                 (* tapp t1 t2 *)
+    (fun y T t1 mt1 =>                                  (* tabs y T t1 *)
+       tabs y T (if eq_id_dec x y then t1 else mt1))
+    (fun r mr => trcd mr)                               (* trcd r *)
+      (nil)                                               (* nil *)
+      (fun i t r mt mr => (Fv i mt) :: mr)                (* cons i t r *)
+    (fun t1 mt1 i => tproj mt1 i)                       (* tproj t1 i *)
+    (fun tb mtb tt mtt te mte => tif mtb mtt mte)       (* tif tb tt te *)
+    .
+
+
+(* Some other stuff: *)
+
+Fixpoint alist_all {T : Type} (P : T-> Prop) (a: alist T) : Prop :=
+  match a with
+    | nil => True
+    | (i, t) :: r => P t /\ alist_all P r
+  end.
+
+Definition tm_rect_nest_map
+  (ftrue : tm)
+  (ffalse : tm)
+  (fvar : id -> tm)
+  (fapp : tm -> tm -> tm -> tm -> tm)
+  (fabs : id -> ty ->  tm -> tm -> tm)
+  (fproj : tm -> tm -> id -> tm)
+  (fif : tm -> tm -> tm -> tm -> tm -> tm -> tm)
+ := tm_xrect
+      (fun _ => tm)  (fun _ => list def) ftrue ffalse fvar fapp fabs
+      (fun r mr => trcd mr) nil (fun i t r mt mr => (Fv i mt) :: mr) fproj fif.
+
+
+Definition subst'' (x:id) (s:tm) : tm -> tm := 
+  tm_rect_nest_map
+    ttrue
+    tfalse
+    (fun y => if eq_id_dec x y then s else (tvar y))
+    (fun t1 mt1 t2 mt2 => tapp mt1 mt2)
+    (fun y T t1 mt1 =>  tabs y T (if eq_id_dec x y then t1 else mt1))
+    (fun t1 mt1 i => tproj mt1 i)
+    (fun tb mtb tt mtt te mte => tif mtb mtt mte).
+
+(*
+Example subst''_ok :substf_ok subst''.
+Proof. unfold substf_ok. repeat split. Qed.
+*)
+
+Definition tm_id : tm -> tm := 
+  tm_xrect (fun _ => tm) (fun _ => list def)
+    ttrue 
+    tfalse
+    (fun y => tvar y)
+    (fun t1 mt1 t2 mt2 => tapp t1 t2)
+    (fun y T t1 mt1 =>  tabs y T t1)
+    (fun r mr => trcd r)
+    (nil)
+    (fun i t r mt mr => (Fv i t) :: r)
+    (fun t1 mt1 i => tproj t1 i)
+    (fun tb mtb tt mtt te mte => tif tb tt te).
+(*
+Example ex_id1 : (tm_id (tapp (tvar f) (tvar a)))
+    =  (tapp (tvar f) (tvar a)).
+Proof. reflexivity. Qed.
+*)
